restructure

authoring/seq.dfy
@@ -1,5 +1,5 @@
-// Uncategorized proof helpers. 
-module Prop {
+// Authoring helpers for sequence data types.
+module Seq {
     function calcMax(s: seq<int>): int
     requires |s| > 0
     {
@@ -52,50 +52,5 @@ module Prop {
     predicate uniformArray<T>(x: seq<T>, val: T) 
     {
         forall i :: 0 <= i < |x| ==> x[i] == val
-    }
-}
-
-module Set {
-    predicate greatestNum(a: set<int>, j: int) {
-        forall i :: i in a ==> j >= i
-    }
-
-    predicate smallestNum(a: set<int>, j: int) {
-        forall i :: i in a ==> j <= i
-    }
-}
-
-// Graph theory related proof helpers.
-module GT {
-    trait Node {}
-
-    trait Edge {
-        var from: Node;
-        var to: Node;
-    }
-
-    trait Graph {
-        var nodes: set<Node>;
-        var edges: set<Edge>;
-    }
-
-    class DAG extends Graph {
-        constructor(nodes: set<Node>, edges: set<Edge>)
-        requires forall i :: i in edges ==> i.from in nodes && i.to in nodes;
-        // Not recursive.
-        requires forall e :: e in edges ==> !exists j :: j == e.from && j == e.to
-        {
-            this.nodes := nodes;
-            this.edges := edges;
-        }
-    }
-
-    class WeightedEdge extends Edge {
-        var weight :int;
-        constructor(from: Node, to: Node, weight: int) {
-            this.from := from;
-            this.to := to;
-            this.weight := weight;
-        }
     }
 }
