authoring/graphs.dfy
@@ -1,0 +1,33 @@
+module GT {
+    trait Node {}
+
+    trait Edge {
+        var from: Node;
+        var to: Node;
+    }
+
+    trait Graph {
+        var nodes: set<Node>;
+        var edges: set<Edge>;
+    }
+
+    class DAG extends Graph {
+        constructor(nodes: set<Node>, edges: set<Edge>)
+        requires forall i :: i in edges ==> i.from in nodes && i.to in nodes;
+        // Not recursive.
+        requires forall e :: e in edges ==> !exists j :: j == e.from && j == e.to
+        {
+            this.nodes := nodes;
+            this.edges := edges;
+        }
+    }
+
+    class WeightedEdge extends Edge {
+        var weight :int;
+        constructor(from: Node, to: Node, weight: int) {
+            this.from := from;
+            this.to := to;
+            this.weight := weight;
+        }
+    }
+}
